BasicLeanDatastructures/GetFreshInhabitant.lean
@@ -1,50 +1,75 @@
--- Gets a fresh element of the type that does not occur in the given list
+/-!
+# GetFreshInhabitant
+
+This file defines a type class `GetFreshInhabitant`
+that provides a single function `GetFreshInhabitant.fresh`.
+This function takes as input a list `l` over a type `t` and then returns an element
+of type `t` that does itself not occur in `l`.
+This captures the intuition that certain types always allow picking "fresh" representants.
+For example, one would assume that it is always possibly to pick a fresh natural numbers if only finitely many numbers have been used so far.
+
+To give an example, we also implement this typeclass for the natural numbers at the end of the file.
+-/
+
+
+/-- A type class that allows to get a fresh element of the desired type. That is, an element that does not occur in a given list. -/
 class GetFreshInhabitant (t : Type u) where
   fresh (l : List t) : { e : t // e ∉ l }
 
-def GetFreshInhabitant.fresh_n {t : Type u} [GetFreshInhabitant t] (l : List t) (n : Nat) :
-    { l' : List t // l'.length = n ∧ l'.Nodup ∧ ∀ e ∈ l', e ∉ l } :=
-  match n with
-  | .zero => ⟨[], by simp⟩
-  | .succ n =>
-    let rec_res := GetFreshInhabitant.fresh_n l n
-    let fresh_e := GetFreshInhabitant.fresh (rec_res.val ++ l)
-    ⟨fresh_e.val :: rec_res.val, by
-      constructor
-      . simp [rec_res.property.left]
-      constructor
-      . rw [List.nodup_cons]
+namespace GetFreshInhabitant
+
+  /-- If we are able to pick individual fresh elements, we can also pick a list of n fresh elements at once using this function. Of course this list shall not contain any duplicates. -/
+  def fresh_n {t : Type u} [GetFreshInhabitant t] (l : List t) (n : Nat) :
+      { l' : List t // l'.length = n ∧ l'.Nodup ∧ ∀ e ∈ l', e ∉ l } :=
+    match n with
+    | .zero => ⟨[], by simp⟩
+    | .succ n =>
+      let rec_res := GetFreshInhabitant.fresh_n l n
+      let fresh_e := GetFreshInhabitant.fresh (rec_res.val ++ l)
+      ⟨fresh_e.val :: rec_res.val, by
         constructor
-        . intro contra
-          apply fresh_e.property
-          rw [List.mem_append]
-          apply Or.inl
-          exact contra
-        . exact rec_res.property.right.left
-      . intro e e_mem
-        rw [List.mem_cons] at e_mem
-        cases e_mem with
-        | inr e_mem => apply rec_res.property.right.right; exact e_mem
-        | inl e_mem =>
-          intro contra
-          apply fresh_e.property
-          rw [List.mem_append]
-          apply Or.inr
-          rw [e_mem] at contra
-          exact contra
+        . simp [rec_res.property.left]
+        constructor
+        . rw [List.nodup_cons]
+          constructor
+          . intro contra
+            apply fresh_e.property
+            rw [List.mem_append]
+            apply Or.inl
+            exact contra
+          . exact rec_res.property.right.left
+        . intro e e_mem
+          rw [List.mem_cons] at e_mem
+          cases e_mem with
+          | inr e_mem => apply rec_res.property.right.right; exact e_mem
+          | inl e_mem =>
+            intro contra
+            apply fresh_e.property
+            rw [List.mem_append]
+            apply Or.inr
+            rw [e_mem] at contra
+            exact contra
+      ⟩
+
+end GetFreshInhabitant
+
+namespace Nat
+
+  /-! We give an example implementation for the natural numbers. -/
+
+  /-- For a list of natural numbers, we can pick a fresh element by taking the successor of the maximal number from the list. -/
+  def fresh (l : List Nat) : { n : Nat // n ∉ l} :=
+    ⟨(l.max?.getD 0).succ, by
+      intro contra
+      have le : (l.max?.getD 0).succ ≤ l.max?.getD 0 := List.le_max?_getD_of_mem contra
+      rw [Nat.succ_le_iff] at le
+      simp at le
     ⟩
 
--- Just using Nat as an example / proof of concept here
-def Nat.fresh (l : List Nat) : { n : Nat // n ∉ l} :=
-  ⟨(l.max?.getD 0).succ, by
-    intro contra
-    have le : (l.max?.getD 0).succ ≤ l.max?.getD 0 := List.le_max?_getD_of_mem contra
-    rw [Nat.succ_le_iff] at le
-    simp at le
-  ⟩
+  instance : GetFreshInhabitant Nat where
+    fresh := Nat.fresh
 
-instance : GetFreshInhabitant Nat where
-  fresh := Nat.fresh
+  -- #eval GetFreshInhabitant.fresh_n [2,27,6,3] 5
 
--- #eval GetFreshInhabitant.fresh_n [2,27,6,3] 5
+end Nat
 
