BasicLeanDatastructures/List/Basic.lean
@@ -1,5 +1,12 @@
 import BasicLeanDatastructures.Set.Basic
 
+/-!
+This file contains a collection definitions and theorems about lists that are not part of Lean's standard library.
+At least when initially writing some of these, suitable variants did not exist or I simply did not find them.
+
+Some cleanup is certainly needed here.
+-/
+
 def List.decidableEqNil : (l : List α) -> Decidable (l = [])
 | .nil => .isTrue rfl
 | .cons hd tl => .isFalse (by simp)
@@ -7,13 +14,17 @@ def List.decidableEqNil : (l : List α) -> Decidable (l = [])
 instance (l : List α) : Decidable (l = []) := l.decidableEqNil
 
 namespace List
+  /-- We can convert a list to a set by defining membership in the set through membership in the list. -/
   def toSet (l : List α) : Set α := fun e => e ∈ l
 
+  /-- Membership does not change across the `toSet` conversion. -/
   theorem mem_toSet {l : List α} {e : α} : e ∈ l.toSet ↔ e ∈ l := by
     simp [toSet, Membership.mem]
 
+  /-- For each valid index, the list element at that index is also in `toSet`. -/
   theorem getElem_mem_toSet (l : List α) (i : Fin l.length) : l[i] ∈ l.toSet := by rw [mem_toSet]; apply List.getElem_mem
 
+  /-- Converting a list to a set and then applying a function to each element is the same as first applyign the function and then converting to the set. -/
   theorem map_toSet_eq_toSet_map {l : List α} {f : α -> β} : l.toSet.map f = (l.map f).toSet := by
     apply Set.ext
     intro e
@@ -32,12 +43,14 @@ namespace List
       rw [List.mem_toSet]
       exact e'_mem
 
+  /-- For each element of `l.toSet`, the mapped version of that element is in the set obtained from the mapped list. -/
   theorem mem_toSet_map_of_mem_toSet {l : List α} {e : α} {f : α -> β} : e ∈ l.toSet -> f e ∈ (l.map f).toSet := by
     intro mem
     rw [← map_toSet_eq_toSet_map]
     apply Set.mem_map_of_mem
     exact mem
 
+  /-- The sum of taking any number of elements from a list cannot exceed the sum over the whole list. -/
   theorem sum_take_le_sum (l : List Nat) (i : Fin (l.length + 1)) : (l.take i.val).sum ≤ l.sum := by
     induction l with
     | nil => simp
@@ -49,19 +62,24 @@ namespace List
         apply Nat.add_le_add_left
         apply ih ⟨i.val, i.isLt⟩
 
+  /-- This function is essentially `List.zipIdx` but the indices are associated with a proof that they are indeed smaller than the length of the list, represented as `Fin`. -/
   def zipIdx_with_lt (l : List α) : List (α × (Fin l.length)) :=
     l.zipIdx.attach.map (fun ⟨pair, h⟩ => (pair.fst, ⟨pair.snd, List.snd_lt_of_mem_zipIdx h⟩))
 
+  /-- The length of `zipIdx_with_lt` is the original length. -/
   theorem length_zipIdx_with_lt (l : List α) : l.zipIdx_with_lt.length = l.length := by unfold zipIdx_with_lt; simp
 
+  /-- The first part of a pair at a given index in `zipIdx_with_lt` corresponds to the list element at the same index. -/
   theorem zipIdx_with_lt_getElem_fst_eq_getElem {l : List α} {index : Nat} (h : index < l.length) : (l.zipIdx_with_lt[index]'(by rw [length_zipIdx_with_lt]; exact h)).fst = l[index] := by
     unfold zipIdx_with_lt
     simp
 
+  /-- The second part of a pair at a given index in `zipIdx_with_lt` is exactly this index (represented as `Fin`). -/
   theorem zipIdx_with_lt_getElem_snd_eq_index {l : List α} {index : Nat} (h : index < l.length) : (l.zipIdx_with_lt[index]'(by rw [length_zipIdx_with_lt]; exact h)).snd = ⟨index, h⟩ := by
     unfold zipIdx_with_lt
     simp
 
+  /-- Membership in `zipIdx_with_lt` is equivalent to membership in `List.zipIdx`. -/
   theorem mem_zipIdx_with_lt_iff_mem_zipIdx {l : List α} : ∀ (i : Fin l.length) (el : α), (el, i) ∈ l.zipIdx_with_lt ↔ (el, i.val) ∈ l.zipIdx := by
     intro i el
     unfold zipIdx_with_lt
@@ -74,14 +92,17 @@ namespace List
           exact h
     . intro h; exists i.val; exists h
 
+  /-- A pair of an element `el` and an index `i` is in `zipIdx_with_lt` if and only if `el` is at index `i` in the underlying list. -/
   theorem mk_mem_zipIdx_with_lt_iff_getElem {l : List α} : ∀ (i : Fin l.length) (el : α), (el, i) ∈ l.zipIdx_with_lt ↔ l[i.val] = el := by
     intro i el
     rw [mem_zipIdx_with_lt_iff_mem_zipIdx]
     rw [List.mk_mem_zipIdx_iff_getElem?]
     simp
 
+  /-- Converts any with a negated predicate into a negated call to all with a positive predicate. -/
   theorem neg_all_of_any_neg (l : List α) (p : α -> Bool) : l.any (fun a => ¬p a) -> ¬l.all p := by simp
 
+  /-- Components of two append calls are equal if the appended lists are equal and the first components have the same length. -/
   theorem append_args_eq_of_append_eq_of_same_length {as bs cs ds : List α} (h : as.length = cs.length) : as ++ bs = cs ++ ds -> as = cs ∧ bs = ds := by
     induction as generalizing cs with
     | nil => cases cs with | nil => simp | cons _ _ => contradiction
@@ -97,10 +118,12 @@ namespace List
           rw [(ih h tail).left]
         . exact (ih h tail).right
 
+  /-- Two lists resulting from append calls are equal if the individual components are equal. -/
   theorem append_eq_append_of_parts_eq (as bs cs ds : List α) : as = cs -> bs = ds -> as ++ bs = cs ++ ds := by
     intro eq eq2
     rw [eq, eq2]
 
+  /-- If two lists resulting from append calls are equal and the second components have the same length, then the first components also have the same length. -/
   theorem append_left_same_length_of_append_eq_append_of_right_same_length {as bs cs ds : List α} : as ++ bs = cs ++ ds -> bs.length = ds.length -> as.length = cs.length := by
     induction as generalizing cs with
     | nil => cases cs with | nil => simp | cons _ _ => simp only [List.nil_append]; intro eq eq2; rw [eq, Nat.eq_iff_le_and_ge] at eq2; have contra := eq2.left; simp only [List.length_append, List.length_cons] at contra; rw [Nat.add_assoc] at contra; apply False.elim; apply Nat.not_succ_le_self; rw [Nat.succ_eq_one_add]; exact Nat.le_of_add_left_le contra
@@ -118,11 +141,13 @@ namespace List
         . rw [List.cons_append, List.cons_append, List.cons_eq_cons] at eq; exact eq.right
         . exact eq2
 
+  /-- A non-empty list can be split into its head and tail. -/
   theorem head_cons_tail_of_ne_nil {l : List α} (h : l ≠ []) : l = (l.head h) :: l.tail := by
     cases l with
     | nil => contradiction
     | cons head tail => simp
 
+  /-- An element is in a list if and only if the list is composable such the element has its first occurrence in this composition. -/
   theorem mem_iff_append_and_not_in_first [DecidableEq α] (l : List α) (e : α) : e ∈ l ↔ ∃ as bs, l = as ++ (e :: bs) ∧ ¬ e ∈ as := by
     induction l with
     | nil => simp
@@ -144,6 +169,8 @@ namespace List
         rcases h with ⟨as, bs, eq, _⟩
         simp [eq]
 
+  /-- Mapping over list produces the same list if the mapping function maps each list member to itself. Note that this is very close to `List.map_id''`
+    but that `List.map_id''` has a stronger assumption. Namely it requires the function to be the id not only on list elements but on every representant of the element type. -/
   theorem map_id_of_id_on_all_mem (l : List α) (f : α -> α) (id_on_all_mem : ∀ e, e ∈ l -> f e = e) : l.map f = l := by
     induction l with
     | nil => simp
@@ -156,6 +183,7 @@ namespace List
         simp [e_mem]
       . simp
 
+  /-- Filtering a list based on two predicates yields the same list if the predicates behave the same on all elements. -/
   theorem filter_eq_of_all_eq (l : List α) (p q : α -> Bool) : (∀ e, e ∈ l -> p e = q e) -> l.filter p = l.filter q := by
     intro h
     induction l with
@@ -182,6 +210,7 @@ namespace List
           simp [this]
         . simp
 
+  /-- Lists over subtypes are equal if and only if their unattached versions are equal. -/
   theorem eq_iff_unattach_eq {α : Type u} {p : α -> Prop} {as bs : List {x : α // p x}} : as.unattach = bs.unattach ↔ as = bs := by
     constructor
     . intro h
@@ -204,6 +233,7 @@ namespace List
     . intro h
       rw [h]
 
+  /-- Erasing an element from a list without duplicates produces a list without duplicates. -/
   theorem nodup_erase_of_nodup [DecidableEq α] (l : List α) (e : α) (nodup : l.Nodup) : (l.erase e).Nodup := by
     induction l with
     | nil => simp [List.erase]
@@ -224,12 +254,13 @@ namespace List
             exact eq
         . exact ih nodup.right
 
+  /-- A list that is longer than a list without duplicates but only contains the same elements must have a duplicate. -/
   theorem contains_dup_of_exceeding_nodup_list_with_same_elements
       [DecidableEq α]
       (as bs : List α)
       (nodup_as : as.Nodup)
       (len_lt : as.length < bs.length)
-      (contains_all : ∀ e, e ∈ bs -> e ∈ as) :
+      (contains_all : bs ⊆ as) :
       ¬ bs.Nodup := by
     induction bs generalizing as with
     | nil => simp at len_lt
@@ -263,14 +294,19 @@ namespace List
             contradiction
         . exact contra.right
 
+  /-- For two equal lists, filter does the same. -/
   theorem filter_eq_of_eq {as bs : List α} : as = bs -> ∀ (f : α -> Bool), as.filter f = bs.filter f := by intro h f; rw [h]
 
+  /-- For two equal lists, map does the same. -/
   theorem map_eq_of_eq {as bs : List α} : as = bs -> ∀ (f : α -> β), as.map f = bs.map f := by intro h f; rw [h]
 
+  /-- For two equal lists, flatten does the same. -/
   theorem flatten_eq_of_eq {as bs : List (List α)} : as = bs -> as.flatten = bs.flatten := by intro h; rw [h]
 
+  /-- Elements at equal indices are the same. -/
   theorem getElem_eq_getElem_of_idx_eq {l : List α} {i j : Nat} {i_lt : i < l.length} (idx_eq : i = j) : l[i] = l[j] := by simp [idx_eq]
 
+  /-- We getting the element at the index of a given element `e`, we obtain exactly `e`. Note that this depends on `LawfulBEq`. -/
   theorem getElem_idxOf_of_mem [BEq α] [LawfulBEq α] {l : List α} {e : α} (mem : e ∈ l) : l[l.idxOf e]'(by apply List.idxOf_lt_length_of_mem; exact mem) = e := by
     induction l with
     | nil => simp at mem
@@ -288,6 +324,7 @@ namespace List
         | inl mem => rw [mem] at neq; simp at neq
         | inr mem => exact mem
 
+  /-- The index of an element that we get from given index is exactly this index. Note that this uses `DecidableEq`. -/
   theorem idxOf_getElem [DecidableEq α] {l : List α} {i : Nat} {lt : i < l.length} (nodup : l.Nodup) : l.idxOf l[i] = i := by
     induction l generalizing i with
     | nil => simp at lt
