BasicLeanDatastructures/List/EraseDupsKeepRight.lean
@@ -1,5 +1,15 @@
+/-!
+# eraseDupsKeepRight
+
+In this file, we define the `eraseDupsKeepRight` convenience function that removes duplicates from a given list while keeping the rightmost occurrence.
+This function assumes `DecidableEq` on the list elements.
+As one would expect, the resulting list is free of duplicates and still contains the same members as the original list, which
+is shown in theorems below.
+-/
+
 namespace List
 
+  /-- If two lists have no duplicates and have the same elements, then their length is the same. Note that the lists are not necessarily equal since the order of elements may differ. -/
   theorem length_eq_of_nodup_of_same_elements [DecidableEq α] (l1 l2 : List α) (nodup1 : l1.Nodup) (nodup2 : l2.Nodup) (same_elems : ∀ e, e ∈ l1 ↔ e ∈ l2) : l1.length = l2.length := by
     induction l1 generalizing l2 with
     | nil =>
@@ -35,10 +45,12 @@ namespace List
           rw [List.mem_cons] at e_mem
           cases e_mem; contradiction; assumption
 
+  /-- Remove duplicates from a list, keeping the rightmost occurrense. -/
   def eraseDupsKeepRight [DecidableEq α] : List α -> List α
   | [] => []
   | hd::tl => if hd ∈ tl then tl.eraseDupsKeepRight else hd::(tl.eraseDupsKeepRight)
 
+  /-- The deduplicated list contains the same elements as the original list. -/
   theorem mem_eraseDupsKeepRight [DecidableEq α] (l : List α) : ∀ e, e ∈ l.eraseDupsKeepRight ↔ e ∈ l := by
     induction l with
     | nil => simp [eraseDupsKeepRight]
@@ -49,6 +61,7 @@ namespace List
       | inl mem => simp [mem]; rw [ih]; simp; intro eq; rw [eq]; exact mem
       | inr not_mem => simp [not_mem]; rw [ih]
 
+  /-- The deduplicated list indeed has no duplicates. -/
   theorem nodup_eraseDupsKeepRight [DecidableEq α] (l : List α) : l.eraseDupsKeepRight.Nodup := by
     induction l with
     | nil => simp [eraseDupsKeepRight]
@@ -58,6 +71,7 @@ namespace List
       | inl mem => simp [mem, ih]
       | inr not_mem => simp [not_mem, ih]; rw [mem_eraseDupsKeepRight]; exact not_mem
 
+  /-- Calling `eraseDupsKeepRight` a second time does not change anything anymore. -/
   theorem eraseDupsKeepRight_idempotent [DecidableEq α] (l : List α) : l.eraseDupsKeepRight.eraseDupsKeepRight = l.eraseDupsKeepRight := by
     induction l with
     | nil => simp [eraseDupsKeepRight]
@@ -74,6 +88,7 @@ namespace List
         simp only [this, ↓reduceIte]
         rw [ih]
 
+  /-- If two lists contain the same elements, then calling `eraseDupsKeepRight` on both ends up with lists of equal length. Again the lists might not be equal as they could differ in their order of elements. -/
   theorem length_eraseDupsKeepRight_eq_of_same_elements [DecidableEq α] (l1 l2 : List α) : (∀ e, e ∈ l1 ↔ e ∈ l2) -> l1.eraseDupsKeepRight.length = l2.eraseDupsKeepRight.length := by
     intro same_elems
     apply length_eq_of_nodup_of_same_elements
