BasicLeanDatastructures/Nat.lean
@@ -1,3 +1,4 @@
+/-- if a there is a natural number such that a certain property holds, then there is a smallest such number. -/
 theorem prop_for_nat_has_minimal_such_nat (prop : Nat -> Prop) : ∀ i, prop i -> (∃ i, prop i ∧ ∀ (j : Fin i), ¬ prop j.val) := by
   intro i h
   -- TODO: can we do this without classical? at least going through all j < i should be possible; only prop might not be decidable
