BasicLeanDatastructures/Set/Basic.lean
@@ -1,3 +1,9 @@
+/-!
+# Set
+
+This file introduces a very basic `Set` type, which is merely a function from the element type into `Prop`.
+-/
+
 def Set (α : Type u) := α -> Prop
 
 instance : EmptyCollection (Set α) where
@@ -17,6 +23,7 @@ instance : HasSSubset (Set α) where
 
 namespace Set
 
+  /-- Two sets are the same if they feature the same elements. -/
   theorem ext (X Y : Set α) : (∀ e, e ∈ X ↔ e ∈ Y) -> X = Y := by
     intro h
     apply funext
@@ -30,6 +37,7 @@ namespace Set
     . apply ext
     . intro h e; rw [h]
 
+  /-- A non-empty set contains at least one element. -/
   theorem not_empty_contains_element (X : Set α) : X ≠ ∅ -> ∃ e, e ∈ X := by
     intro neq
     apply Classical.byContradiction
@@ -42,16 +50,20 @@ namespace Set
     simp only [contra, false_iff]
     simp [Membership.mem, EmptyCollection.emptyCollection]
 
+  /-- Apply a mapping function to each member of a set yielding a new set; think of `List.map`. -/
   def map (X : Set α) (f : α -> β) : Set β := fun e => ∃ e', e' ∈ X ∧ e = f e'
 
+  /-- For a set element, the mapped version of the element is in the mapped set. -/
   theorem mem_map_of_mem {e : α} {X : Set α} {f : α -> β} : e ∈ X -> f e ∈ X.map f := by
     intros
     exists e
 
+  /-- The subset relation on sets is reflexive. -/
   theorem subset_refl {X : Set α} : X ⊆ X := by
     intros _ h
     exact h
 
+  /-- The subset relation on sets is transitive. -/
   theorem subset_trans {a b c : Set α} : a ⊆ b -> b ⊆ c -> a ⊆ c := by
     intro ha hb
     intro e he
@@ -59,18 +71,21 @@ namespace Set
     apply ha
     assumption
 
+  /-- When a is a subset of b, then a is still a subset of the union of b with c. -/
   theorem subset_union_of_subset_left {a b c : Set α} : a ⊆ b -> a ⊆ b ∪ c := by
     intro aSubB e eInA
     apply Or.inl
     apply aSubB
     exact eInA
 
+  /-- When a is a subset of c, then a is still a subset of the union of b with c. -/
   theorem subset_union_of_subset_right (a b c : Set α) : a ⊆ c -> a ⊆ b ∪ c := by
     intro aSubC e eInA
     apply Or.inr
     apply aSubC
     exact eInA
 
+  /-- The union of a and b is a subset of c if and only if a and b are both subsets of c. -/
   theorem union_subset_iff_both_subset (a b c : Set α) : a ∪ b ⊆ c ↔ a ⊆ c ∧ b ⊆ c := by
     constructor
     . intro h
