BasicLeanDatastructures/Set/Finite.lean
@@ -2,16 +2,26 @@ import BasicLeanDatastructures.Set.Basic
 import BasicLeanDatastructures.List.Basic
 import BasicLeanDatastructures.List.EraseDupsKeepRight
 
+/-!
+# Set.finite
+
+This file handles a simple definition for when a set is considered finite, namely
+when there exists a list that contains the same elements.
+-/
+
 namespace Set
 
+  /-- A set is finite if there is a list with the same elements. We also enforce this list to be free of duplicates right now but this might change in the future. -/
   def finite (X : Set α) : Prop := ∃ (l : List α), l.Nodup ∧ ∀ (e : α), e ∈ l ↔ e ∈ X
 
+  /-- To show that a Set is finite, it is enough to give a list with the same elements not caring about duplicates. Duplicates are removed using `List.eraseDupsKeepRight` internally. -/
   theorem finite_of_list_with_same_elements [DecidableEq α] {X : Set α} (l : List α) (same_elements : ∀ e, e ∈ l ↔ e ∈ X) : X.finite := by
     exists l.eraseDupsKeepRight
     constructor
     . apply l.nodup_eraseDupsKeepRight
     . intro e; rw [l.mem_eraseDupsKeepRight, same_elements]
 
+  /-- Subsets of finite sets are finite. -/
   theorem finite_of_subset_finite [DecidableEq α] {a b : Set α} (fin : b.finite) : a ⊆ b -> a.finite := by
     intro sub
     rcases fin with ⟨l, _, l_eq⟩
@@ -23,12 +33,13 @@ namespace Set
     . apply List.nodup_eraseDupsKeepRight
     . intro e
       rw [List.mem_eraseDupsKeepRight, List.mem_filter]
-      simp
+      simp only [decide_eq_true_eq, and_iff_right_iff_imp]
       intro e_mem
       rw [l_eq]
       apply sub
       exact e_mem
 
+  /-- Unions of finite sets are finite. -/
   theorem union_finite_of_both_finite [DecidableEq α] {a b : Set α} (fin_a : a.finite) (fin_b : b.finite) : (a ∪ b).finite := by
     rcases fin_a with ⟨l, _, l_eq⟩
     rcases fin_b with ⟨k, _, k_eq⟩
@@ -52,6 +63,7 @@ end Set
 
 namespace List
 
+  /-- Sets obtained from lists are finite. -/
   theorem finite_toSet [DecidableEq α] (l : List α) : l.toSet.finite := by
     apply Set.finite_of_list_with_same_elements l
     intro e
